---
title: "Ito Calculus"
author: "Quasar"
date: "2024-07-12"
categories: [Stochastic Calculus]      
image: "image.jpg"
toc: true
toc-depth: 3
---

## Exercises

::: {#exr-a-strange-martingale}

(A strange martingale) Let $(B_t,t\geq 0)$ be a standard Brownian motion. Consider the process:

$$
M_t = \frac{1}{\sqrt{1-t}}\exp\left(\frac{-B_t^2}{2(1-t)}\right), \quad \text{ for }0 \leq t < 1
$$

(a) Show that $M_t$ can be represented by:

$$
M_t = 1 + \int_0^t \frac{-B_s M_s}{1-s}dB_s, \quad \text{ for } 0 \leq t \leq 1
$$

(b) Deduce from the previous question that $(M_s,s \leq t)$ is a martingale for $t < 1$ and for the Brownian filtration.

(c) Show that $\mathbb{E}[M_t] = 1$ for all $t < 1$.

(d) 
:::

*Solution*.

Let $f(t,x) = \frac{1}{\sqrt{1-t}}e^{-\frac{x^2}{2(1-t)}}$. We have:

$$
\begin{align*}
\frac{\partial f}{\partial t} &= \frac{\sqrt{1-t}\cdot e^{-\frac{x^2}{2(1-t)}}\cdot \frac{x^2}{2(1-t)^2}\cdot (-1) - e^{-\frac{x^2}{2(1-t)}}\cdot \frac{1}{2\sqrt{1-t}}\cdot(-1)}{(1-t)}\\
&=\frac{e^{-\frac{x^2}{2(1-t)}}}{(1-t)}\left( -\frac{x^2}{2(1-t)^{3/2}}+\frac{1-t}{2(1-t)^{3/2}}\right)\\
&= \frac{e^{-\frac{x^2}{2(1-t)}}((1-t) - x^2)}{2(1-t)^{5/2}}
\end{align*}
$$

Also, the first and second derivatives with respect to the space variable $x$ are:

$$
\begin{align*}
\frac{\partial f}{\partial x} &= \frac{1}{\sqrt{1-t}}\exp\left(-\frac{x^2}{2(1-t)}\right)\left(-\frac{x}{(1-t)}\right)\\
&= -\frac{x}{(1-t)^{3/2}} \exp\left(-\frac{x^2}{2(1-t)}\right)
\end{align*}
$$

$$
\begin{align*}
\frac{\partial^2 f}{\partial x^2} &= - \frac{1}{(1-t)^{3/2}}\left\{\exp\left(-\frac{x^2}{2(1-t)}\right) + x\exp\left(-\frac{x^2}{2(1-t)}\right)\left(-\frac{x}{(1-t)}\right)\right\}\\
&= - \frac{1}{(1-t)^{3/2}}\exp\left(-\frac{x^2}{2(1-t)}\right) \left\{1 - \frac{x^2}{(1-t)}\right\}\\
&= \frac{(x^2 - (1-t))}{(1-t)^{5/2}}\exp\left(-\frac{x^2}{2(1-t)}\right)
\end{align*}
$$

By Ito's formula:

$$
\begin{align*}
df(t,B_t) &= (f_t + \frac{1}{2}f_{xx})dt + f_x dB_t\\
dM_t &= -\frac{B_t}{(1-t)} \frac{e^{-\frac{B_t^2}{2(1-t)}}}{\sqrt{1-t}}\\
&= -\frac{B_t M_t}{(1-t)}
\end{align*}
$$

where in the second step, we used the fact that $f_t + \frac{1}{2}f_{xx} = 0$, so the $dt$ term is zero.

In the integral form:

$$
\begin{align*}
M_t - M_0 &= \int \frac{- B_s M_s}{1 - s}dB_s\\
M_t &= 1 + \int \frac{- B_s M_s}{1 - s}dB_s
\end{align*}
$$

(b) The Ito integral $\int_0^t \frac{-B_s M_s}{1-s}dB_s$ is a continuous martingale with respect to the brownian filtration. Hence $(M_t,t \geq 0)$ is a martingale.

(c) The expectation of an Ito integral is zero. Hence, $\mathbb{E}[M_t] = 1$ for all $t < 1$.

(d)

